Saving some monad modification work

theories/Monad.v
@@ -10,40 +10,48 @@ From CVM Require Export Attestation_Session St IO_Axioms Utils.
 From CVM Require Import Interface.Interface.
 
 (** * CVM monadic primitive operations *)
+Create HintDb cvm.
 
 Definition get_st : CVM cvm_st :=
-  st_conf <~ get ;;;
-  match st_conf with
-  | (st, conf) => ret st
-  end.
+  ↑cs (
+    st <- get ;;s
+    ↑sr (res st)
+  ).
+Hint Unfold get_st : cvm.
 
 Definition get_config : CVM Session_Config :=
-  st_conf <~ get ;;;
-  match st_conf with
-  | (st, conf) => ret conf
-  end.
+  conf <- ask ;;c
+  ↑cs (
+    ↑sr (res conf)
+  ).
+Hint Unfold get_config : cvm.
 
 Definition get_trace : CVM (list Ev) :=
-  st <~ get_st ;;;
+  st <- get_st ;;;c
   ret (st_trace st).
+Hint Unfold get_trace : cvm.
 
 Definition get_evid : CVM Event_ID :=
   st <~ get_st ;;;
   ret (st_evid st).
+Hint Unfold get_evid : cvm.
 
 Definition put_trace (tr' : list Ev) : CVM unit :=
   i <~ get_evid ;;;
   conf <~ get_config ;;;
   put (mk_st tr' i, conf).
+Hint Unfold put_trace : cvm.
 
 Definition put_evid (i' : Event_ID) : CVM unit :=
   tr <~ get_trace ;;;
   conf <~ get_config ;;;
   put (mk_st tr i', conf).
+Hint Unfold put_evid : cvm.
 
 Definition get_pl : CVM Plc :=
   sc <~ get_config ;;;
   ret (session_plc sc).
+Hint Unfold get_pl : cvm.
 
 Definition inc_id : CVM Event_ID :=
   tr <~ get_trace ;;;
@@ -51,10 +59,12 @@ Definition inc_id : CVM Event_ID :=
   conf <~ get_config ;;;
   put (mk_st tr (Nat.add i 1), conf) ;;;
   ret i.
+Hint Unfold inc_id : cvm.
 
 Definition add_trace (tr:list Ev) : CVM unit :=
   tr' <~ get_trace ;;;
   put_trace (tr' ++ tr).
+Hint Unfold add_trace : cvm.
 
 (* TODO: consider removing split/join events from reference semantics.
          Would make this (no-op) helper unecessary. *)
@@ -62,6 +72,7 @@ Definition split_ev : CVM unit :=
   p <~ get_pl ;;;
   i <~ inc_id ;;;
   add_trace [Term_Defs.split i p].
+Hint Unfold split_ev : cvm.
 
 (** * Partially-symbolic implementations of IO operations *)
 
@@ -72,6 +83,7 @@ Definition tag_ASP (params :ASP_PARAMS) (mpl:Plc) (e:Evidence) : CVM Event_ID :=
   x <~ inc_id ;;;
   add_trace [umeas x mpl params (get_et e)] ;;;
   ret x.
+Hint Unfold tag_ASP : cvm.
 
 Local Open Scope list_scope.
 
@@ -82,39 +94,42 @@ Definition join_seq (e1:Evidence) (e2:Evidence): CVM Evidence :=
   let '(evc bits2 et2) := e2 in
   add_trace [join n p] ;;;
   ret (evc (bits1 ++ bits2) (split_evt et1 et2)).
+Hint Unfold join_seq : cvm.
 
 Definition hoist_result {A : Type} (r : Result A string) : CVM A :=
   match r with
   | res a => ret a
   | err e => fail (dispatch_error (Runtime e))
   end.
+Hint Unfold hoist_result : cvm.
 
 Definition hoist_option {A : Type} (o : option A) (msg : string) : CVM A :=
   match o with
   | Some a => ret a
   | None => fail (dispatch_error (Runtime msg))
   end.
+Hint Unfold hoist_option : cvm.
 
-Definition get_asp_type (a : ASP_ID) : CVM EvSig :=
+Definition get_asp_type `{DecEq ASP_ID} (a : ASP_ID) : CVM EvSig :=
   sc <~ get_config ;;;
   let G := session_context sc in
   hoist_option ((asp_types G) ![ a ]) err_str_asp_no_type_sig.
+Hint Unfold get_asp_type : cvm.
 
-Definition get_asp_dual (a : ASP_ID) : CVM ASP_ID :=
+Definition get_asp_dual `{DecEq ASP_ID} (a : ASP_ID) : CVM ASP_ID :=
   sc <~ get_config ;;;
   let G := session_context sc in
   hoist_option ((asp_comps G) ![ a ]) err_str_asp_no_compat_appr_asp.
+Hint Unfold get_asp_dual : cvm.
 
-(* Helper function that builds a new internal EvidenceT bundle based on 
-   the EvidenceT extension parameter of an ASP term. *)
-Definition bundle_asp (p:Plc) (rwev : RawEv) 
+Definition bundle_asp `{DecEq nat, DecEq ASP_ID} (p:Plc) (rwev : RawEv) 
     (cur_ev : Evidence) (ps:ASP_PARAMS) : CVM Evidence :=
   let '(asp_paramsC asp_id args targ_plc targ) := ps in
   '(ev_arrow fwd in_sig out_sig) <~ get_asp_type asp_id ;;;
   match out_sig with
   | (OutN n) =>
-    if (dec_eq (List.length rwev) n)
-    then 
+    match (dec_eq (List.length rwev) n) with
+    | left _ => 
       match fwd with
 (* The semantics for a "REPLACE" asp are it CONSUMES all incoming evidence,
 then returns a new collection of evidence that will REPLACE the CVMs current 
@@ -133,7 +148,10 @@ current CVM evidence bundle *)
         | evc bits et => ret (evc (rwev ++ bits) (asp_evt p ps et))
         end
       end
-    else fail (dispatch_error (Runtime errStr_raw_EvidenceT_too_long))
+    | right _ => 
+      (* we are not the right size, so we fail *)
+      fail (dispatch_error (Runtime errStr_raw_EvidenceT_too_long))
+    end
   | OutUnwrap =>
     match fwd with
     | WRAP => fail (dispatch_error (Runtime err_str_only_unwrap_can_be_outwrap))
@@ -146,9 +164,11 @@ current CVM evidence bundle *)
       size_below_wrap' <~ hoist_result (apply_to_evidence_below G (et_size G) [Trail_UNWRAP asp_id] et) ;;;
       size_below_wrap <~ hoist_result (size_below_wrap' ) ;;;
       (* we now need to just verify that we are the same size as what was below the wrap *)
-      if (dec_eq (List.length rwev) size_below_wrap)
-      then ret (evc rwev (asp_evt p ps et))
-      else fail (dispatch_error (Runtime err_str_unwrap_of_wrap_same_size))
+      match (dec_eq (List.length rwev) size_below_wrap) with
+      | left _ => ret (evc rwev (asp_evt p ps et))
+      | right _ =>
+        fail (dispatch_error (Runtime err_str_unwrap_of_wrap_same_size))
+      end
       (* match r with
       | asp_evt p' (asp_paramsC wrap_id _ _ _) et' =>
         '(ev_arrow fwd _ _) <~ get_asp_type wrap_id ;;;
@@ -169,6 +189,7 @@ current CVM evidence bundle *)
       end *)
     end
   end.
+Hint Unfold bundle_asp : cvm.
 
 (** * Stub for invoking external ASP procedures.  
       Extracted code should not need to use the Plc or Event_ID parameters 
@@ -179,20 +200,22 @@ Definition do_asp (params :ASP_PARAMS) (e:RawEv) (x:Event_ID) : CVM RawEv :=
   | res r => ret r
   | err e => fail (dispatch_error e)
   end.
+Hint Unfold do_asp : cvm.
 
 (* Simulates invoking an arbitrary ASP.  Tags the event, builds and returns 
    the new EvidenceT bundle. *)
-Definition invoke_ASP (e : Evidence) (params : ASP_PARAMS) : CVM Evidence :=
+Definition invoke_ASP `{DecEq ASP_ID} (e : Evidence) (params : ASP_PARAMS) : CVM Evidence :=
   p <~ get_pl ;;;
   x <~ tag_ASP params p e ;;;
   rawev <~ do_asp params (get_bits e) x ;;;
   outev <~ bundle_asp p rawev e params ;;;
   ret outev.
+Hint Unfold invoke_ASP : cvm.
 
 (* Simulates invoking an arbitrary ASP.  Tags the event, builds and returns 
    the new EvidenceT bundle. *)
 
-Fixpoint invoke_APPR' (r : RawEv) (et : EvidenceT) (out_evt : EvidenceT) {struct et} : CVM Evidence :=
+Fixpoint invoke_APPR' `{DecEq ASP_ID} (r : RawEv) (et : EvidenceT) (out_evt : EvidenceT) {struct et} : CVM Evidence :=
   sc <~ get_config ;;;
   let G := (session_context sc) in
   match et with
@@ -213,11 +236,12 @@ Fixpoint invoke_APPR' (r : RawEv) (et : EvidenceT) (out_evt : EvidenceT) {struct
       (* Check that the "UNWRAP" occured properly *)
       n' <~ hoist_result (et_size G et'') ;;;
       n'' <~ hoist_result (et_size G et') ;;;
-      if (dec_eq n' n'')
-      then (* The "UNWRAP" worked *)
+      match (dec_eq n' n'') with
+      | right _ => fail (dispatch_error (Runtime err_str_appr_wrap_failed))
+      | left _ => (* The "UNWRAP" worked *)
         (* so do the recursive call *)
         invoke_APPR' r'' et' (asp_evt (session_plc sc) dual_par out_evt)
-      else fail (dispatch_error (Runtime err_str_appr_wrap_failed))
+      end
     | UNWRAP =>
       (* to appraise an UNWRAP is to appraise whatever is below 
       the UNWRAP and WRAP *)
@@ -287,15 +311,18 @@ Fixpoint invoke_APPR' (r : RawEv) (et : EvidenceT) (out_evt : EvidenceT) {struct
 
 Definition invoke_APPR (e : Evidence) : CVM Evidence :=
   invoke_APPR' (get_bits e) (get_et e) (get_et e).
+Hint Unfold invoke_APPR : cvm.
 
 Definition nullEv : CVM Evidence :=
   p <~ get_pl ;;;
   x <~ inc_id ;;;
   add_trace [null x p] ;;;
   ret mt_evc.
+Hint Unfold nullEv : cvm.
 
 Definition clearEv : unit -> CVM Evidence :=
   fun _ => ret mt_evc.
+Hint Unfold clearEv : cvm.
 
 (* Helper that interprets primitive core terms in the CVM.  *)
 Definition do_prim (e : Evidence) (a: ASP) : CVM Evidence :=
@@ -307,6 +334,7 @@ Definition do_prim (e : Evidence) (a: ASP) : CVM Evidence :=
   | APPR => invoke_APPR e 
   | ENC q => invoke_ASP e (enc_params q)
   end.
+Hint Unfold do_prim : cvm.
 
 (* Monadic helper function to simulate a span of remote event IDs 
    corresponding to the size of a Term *)
@@ -316,6 +344,7 @@ Definition inc_remote_event_ids (e : Evidence) (t:Term) : CVM unit :=
   p <~ get_pl ;;;
   n <~ hoist_result (events_size (session_context sc) p (get_et e) t) ;;;
   put_evid (Nat.add i n).
+Hint Unfold inc_remote_event_ids : cvm.
 
 (* Monadic helper function to simulate a span of parallel event IDs 
    corresponding to the size of a Term *)
@@ -325,6 +354,7 @@ Definition inc_par_event_ids (e : Evidence) (t: Term) : CVM unit :=
   p <~ get_pl ;;;
   n <~ hoist_result (events_size (session_context sc) p (get_et e) t) ;;;
   put_evid (Nat.add i n).
+Hint Unfold inc_par_event_ids : cvm.
   
 (* Primitive monadic communication primitives 
    (some rely on Admitted IO Stubs). *)
@@ -332,14 +362,17 @@ Definition inc_par_event_ids (e : Evidence) (t: Term) : CVM unit :=
 Definition tag_REQ (t:Term) (p:Plc) (q:Plc) (e:Evidence) : CVM unit :=
   reqi <~ inc_id ;;;
   add_trace [req reqi p q (get_et e) t].
+Hint Unfold tag_REQ : cvm.
 
 Definition tag_RPY (p:Plc) (q:Plc) (e:Evidence) : CVM unit :=
   rpyi <~ inc_id ;;;
   add_trace [rpy rpyi p q (get_et e)].
+Hint Unfold tag_RPY : cvm.
 
 Definition get_cvm_policy : CVM PolicyT := 
   sc <~ get_config ;;;
   ret (policy sc).
+Hint Unfold get_cvm_policy : cvm.
 
 (* Remote communication primitives *)
 
@@ -370,6 +403,7 @@ Definition do_remote (sc : Session_Config) (pTo: Plc) (e : Evidence) (t:Term)
       end
   | None => err (dispatch_error Unavailable)
   end.
+Hint Unfold do_remote : cvm.
 
 Definition doRemote_session' (pTo:Plc) (e:Evidence) (t:Term) 
     : CVM Evidence := 
@@ -379,6 +413,7 @@ Definition doRemote_session' (pTo:Plc) (e:Evidence) (t:Term)
   | res e' => ret e'
   | err s => fail s
   end.
+Hint Unfold doRemote_session' : cvm.
 
 Definition remote_session (p:Plc) (q:Plc) (e:Evidence) (t:Term) : CVM Evidence :=
   tag_REQ t p q e ;;;
@@ -392,12 +427,14 @@ Definition remote_session (p:Plc) (q:Plc) (e:Evidence) (t:Term) : CVM Evidence :
   add_trace rem_evs ;;;
   inc_remote_event_ids e t ;;;
   ret e'.
+Hint Unfold remote_session : cvm.
 
 Definition doRemote (q:Plc) (e:Evidence) (t:Term) : CVM Evidence :=
   p <~ get_pl ;;;
   e' <~ remote_session p q e t ;;;
   tag_RPY p q e' ;;;
   ret e'.
+Hint Unfold doRemote : cvm.
 
 (* Primitive monadic parallel CVM thread primitives 
    (some rely on Admitted IO Stubs). *)
@@ -409,12 +446,14 @@ Definition start_par_thread (e:Evidence) (t: Term) : CVM nat :=
   do_start_par_thread i e t ;;;
   add_trace [cvm_thread_start i i p (get_et e) t] ;;;
   ret i.
+Hint Unfold start_par_thread : cvm.
 
 Definition do_wait_par_thread (loc:Loc) (p:Plc) (e:Evidence) (t: Term) : CVM Evidence :=
   match (parallel_vm_thread loc p e t) with
   | res e' => ret e'
   | err s => fail s
   end.
+Hint Unfold do_wait_par_thread : cvm.
 
 Definition wait_par_thread (loc:Loc) (e:Evidence) (t: Term) : CVM Evidence :=
   p <~ get_pl ;;;
@@ -430,30 +469,8 @@ Definition wait_par_thread (loc:Loc) (e:Evidence) (t: Term) : CVM Evidence :=
   i <~ inc_id ;;;
   add_trace [cvm_thread_end i loc] ;;;
   ret e'.
-   
-Create HintDb cvm.
-Hint Unfold do_prim : cvm.
-Hint Unfold doRemote : cvm.
-Hint Unfold remote_session : cvm.
-Hint Unfold doRemote_session' : cvm.
-Hint Unfold invoke_ASP : cvm.
-Hint Unfold get_asp_type : cvm.
-Hint Unfold get_asp_dual : cvm.
-Hint Unfold bundle_asp : cvm.
-Hint Unfold do_asp : cvm.
-Hint Unfold clearEv : cvm.
-Hint Unfold nullEv : cvm.
-Hint Unfold hoist_result : cvm.
-Hint Unfold hoist_option : cvm.
-Hint Unfold inc_remote_event_ids : cvm.
-Hint Unfold inc_par_event_ids : cvm.
 Hint Unfold wait_par_thread : cvm.
-Hint Unfold do_wait_par_thread : cvm.
-Hint Unfold join_seq : cvm.
-Hint Unfold get_st : cvm.
-Hint Unfold get_pl : cvm.
-Hint Unfold get_evid : cvm.
-Hint Unfold put_evid : cvm.
-Hint Unfold get_config : cvm.
-Hint Unfold add_trace : cvm.
-Hint Unfold put_trace : cvm.
+
+(* Some other hints relevant to CVM *)
+Hint Unfold get_et : cvm.
+Hint Unfold get_bits : cvm.
